atomics/acq_rel_atomics.v
@@ -59,6 +59,8 @@ Ltac prove_objective := repeat
 Hint Resolve emp_objective data_at_objective own_objective prop_objective andp_objective exp_objective
   sepcon_objective sepcon_list_objective : objective.
 
+
+
 Section dup.
 
 Definition duplicable P := P |-- |==> P * P.
@@ -82,6 +84,11 @@ Hint Resolve sepcon_duplicable : dup.
 Lemma sepcon_list_duplicable : forall lP, Forall duplicable lP -> duplicable (fold_right sepcon emp lP).
 Proof.
   induction 1; simpl; auto with dup.
+Qed.
+
+Lemma iter_sepcon_duplicable : forall {B} (f : B -> mpred) l, (forall a, duplicable (f a)) -> duplicable (iter_sepcon f l).
+Proof.
+  induction l; simpl; auto with dup.
 Qed.
 
 Lemma list_duplicate : forall Q lP, duplicable Q ->
@@ -133,6 +140,8 @@ Definition weak_dup P := P -* |==> (P * P).
 
 End dup.
 
+End inv.
+
 Hint Resolve emp_duplicable sepcon_duplicable invariant_duplicable' ghost_snap_duplicable prop_duplicable : dup.
 
 Section atomics.
@@ -181,8 +190,9 @@ Axiom protocol_A_join' : forall l s1 s2,
   protocol_A l s1 ord T * protocol_A l s2 ord T |--
   EX s : _, !!(ord s1 s /\ ord s2 s) && protocol_A l s ord T.
 
-Axiom make_protocol : forall {P : protocol Tread Tfull} l v s, repable_signed v ->
-  data_at Tsh tint (vint v) l * |> Tfull s v |-- |==> protocol_A l s ord T.
+Axiom make_protocol : forall {P : protocol Tread Tfull} sh l v s,
+  writable_share sh -> repable_signed v ->
+  data_at sh tint (vint v) l * |> Tfull s v |-- |==> protocol_A l s ord T.
 
 Axiom protocol_A_later : forall l s,
   protocol_A l s ord (|>Tread, |>Tfull) |-- |>protocol_A l s ord T.
@@ -220,19 +230,19 @@ Qed.
 Definition OrdType s := ArrowType s (ArrowType s (ConstType Prop)).
 Definition PredType s := ArrowType s (ArrowType (ConstType Z) Mpred).
 
-Definition LA_type := ProdType (ProdType (ProdType (ProdType (ProdType (ProdType
+Definition LA_type := ProdType (ProdType (ProdType (ProdType (ProdType (ProdType (ProdType
   (ConstType val) (DependentType 0)) (OrdType (DependentType 0)))
   (ProdType (PredType (DependentType 0)) (PredType (DependentType 0))))
-  Mpred) (ConstType (iname -> Prop))) (PredType (DependentType 0)).
+  Mpred) (ConstType (iname -> Prop))) (PredType (DependentType 0))) (ConstType invG).
 
 Program Definition load_acq_spec := TYPE LA_type
   WITH l : val, s : _, st_ord : _ -> _ -> Prop, T : ((_ -> Z -> mpred) * (_ -> Z -> mpred)),
-       P : mpred, E : Ensemble iname, Q : _ -> Z -> mpred
+       P : mpred, E : Ensemble iname, Q : _ -> Z -> mpred, inv_names : invG
   PRE [ 1%positive OF tptr tint ]
    PROP ()
    LOCAL (temp 1%positive l)
-   SEP (ALL s' : _, !!(st_ord s s') --> ALL v : _,
-          ((fst T s' v * P * protocol_A l s' st_ord T) -* |={E}=> Q s' v) && emp;
+   SEP ((ALL s' : _, !!(st_ord s s') --> ALL v : _,
+          (fst T s' v * P * protocol_A l s' st_ord T) -* |={E}=> Q s' v) && cored;
         P; protocol_A l s st_ord T)
   POST [ tint ]
    EX v : Z, EX s' : _,
@@ -242,33 +252,33 @@ Program Definition load_acq_spec := TYPE LA_type
 Next Obligation.
 Proof.
   repeat intro.
-  destruct x as ((((((?, s), ?), (?, ?)), P), ?), Q); simpl.
+  destruct x as (((((((?, s), ?), (?, ?)), P), ?), Q), ?); simpl.
   unfold PROPx, LOCALx, SEPx; simpl; rewrite !approx_andp; f_equal;
     f_equal; rewrite !sepcon_emp, ?approx_sepcon, ?approx_idem.
   rewrite protocol_A_super_non_expansive; f_equal.
+  rewrite !approx_andp; f_equal.
   rewrite !approx_allp by auto; f_equal; extensionality.
   setoid_rewrite approx_imp; f_equal; f_equal.
   rewrite !(approx_allp _ _ _ 0); f_equal; extensionality.
-  rewrite !approx_andp; f_equal.
   setoid_rewrite fview_shift_nonexpansive.
   rewrite !approx_sepcon, !approx_idem, protocol_A_super_non_expansive; auto.
 Qed.
 Next Obligation.
 Proof.
   repeat intro.
-  destruct x as ((((((?, ?), ?), ?), ?), ?), ?); simpl.
+  destruct x as (((((((?, ?), ?), ?), ?), ?), ?), ?); simpl.
   rewrite !approx_exp; apply f_equal; extensionality.
   rewrite !approx_exp; apply f_equal; extensionality.
   unfold PROPx, LOCALx, SEPx; simpl; rewrite !approx_andp; do 2 apply f_equal;
     rewrite !sepcon_emp, ?approx_sepcon, ?approx_idem; auto.
 Qed.
 
-Definition SR_type := ProdType (ProdType (ProdType (ProdType (ProdType (ProdType (ProdType
+(*Definition SR_type := ProdType (ProdType (ProdType (ProdType (ProdType (ProdType (ProdType
   (ConstType (val * Z)) (DependentType 0)) (DependentType 0)) (OrdType (DependentType 0)))
   (ProdType (PredType (DependentType 0)) (PredType (DependentType 0))))
   Mpred) (ConstType (iname -> Prop))) Mpred.
 
-(*Program Definition store_rel_spec := TYPE SR_type
+Program Definition store_rel_spec := TYPE SR_type
   WITH l : val, v : Z, s : _, s'' : _, st_ord : _ -> _ -> Prop, T : ((_ -> Z -> mpred) * (_ -> Z -> mpred)),
        P : mpred, II : Z -> mpred, lI : list Z, Q' : mpred, Q : mpred
   PRE [ 1%positive OF tptr tint, 2%positive OF tint ]
@@ -390,23 +400,23 @@ Proof.
   intros; simpl; rewrite invariant_super_non_expansive; auto.
 Qed.*)
 
-Definition CRA_type := ProdType (ProdType (ProdType (ProdType (ProdType
+Definition CRA_type := ProdType (ProdType (ProdType (ProdType (ProdType (ProdType
   (ProdType (ProdType (ConstType (val * Z * Z)) (DependentType 0)) (OrdType (DependentType 0)))
   (ProdType (PredType (DependentType 0)) (PredType (DependentType 0)))) Mpred)
   (ConstType (iname -> Prop))) (ArrowType (DependentType 0) Mpred))
-  (PredType (DependentType 0)).
+  (PredType (DependentType 0))) (ConstType invG).
 
 Program Definition CAS_RA_spec := TYPE CRA_type
   WITH l : val, c : Z, v : Z, s : _, st_ord : _ -> _ -> Prop, T : ((_ -> Z -> mpred) * (_ -> Z -> mpred)),
-       P : mpred, E : _, Q : _ -> mpred, R : _ -> Z -> mpred
+       P : mpred, E : _, Q : _ -> mpred, R : _ -> Z -> mpred, inv_names : invG
   PRE [ 1%positive OF tptr tint, 2%positive OF tint, 3%positive OF tint ]
    PROP (repable_signed c; repable_signed v)
    LOCAL (temp 1%positive l; temp 2%positive (vint c); temp 3%positive (vint v))
    SEP (ALL s' : _, !!(st_ord s s') --> ((snd T s' c * P) -* |={E}=>
-          (EX s'' : _, !!(st_ord s' s'') && |> snd T s'' v *
-           ((protocol_A l s'' st_ord T) -* |={E}=>(Q s'')) && emp)) && emp;
-        ALL s' : _, ALL v' : _, !!(st_ord s s' /\ repable_signed v' /\ v <> c) -->
-          ((|> fst T s' v' * protocol_A l s' st_ord T * P) -* |={E}=> (R s' v')) && emp;
+          (EX s'' : _, !!(st_ord s' s'') && (protocol_A l s'' st_ord T) -* |={E}=> |> snd T s'' v *
+           Q s'')) && cored; (* is this right? *)
+        ALL s' : _, ALL v' : _, !!(st_ord s s' /\ repable_signed v' /\ v' <> c) -->
+          ((|> fst T s' v' * protocol_A l s' st_ord T * P) -* |={E}=> (R s' v')) && cored;
         protocol_A l s st_ord T; P)
   POST [ tint ]
    EX v' : Z, EX s' : _,
@@ -416,7 +426,7 @@ Program Definition CAS_RA_spec := TYPE CRA_type
 Next Obligation.
 Proof.
   repeat intro.
-  destruct x as (((((((((?, ?), ?), s), ?), (?, ?)), ?), ?), ?), ?); simpl.
+  destruct x as ((((((((((?, ?), ?), s), ?), (?, ?)), ?), ?), ?), ?), ?); simpl.
   unfold PROPx; simpl; rewrite !approx_andp; f_equal.
   unfold LOCALx; simpl; rewrite !approx_andp; f_equal.
   unfold SEPx; simpl; rewrite !sepcon_emp, !approx_sepcon, !approx_idem.
@@ -427,13 +437,13 @@ Proof.
     setoid_rewrite fview_shift_nonexpansive.
     rewrite !approx_sepcon, !approx_idem; f_equal; f_equal; f_equal.
     rewrite !approx_exp; f_equal; extensionality.
-    rewrite !approx_andp, !approx_sepcon, !approx_andp; f_equal; f_equal.
-    + f_equal.
+    rewrite wand_nonexpansive; setoid_rewrite wand_nonexpansive at 3; f_equal; f_equal.
+    + rewrite !approx_andp, protocol_A_super_non_expansive; reflexivity.
+    + rewrite fupd_nonexpansive; setoid_rewrite fupd_nonexpansive at 2; f_equal; f_equal.
+      rewrite !approx_sepcon, approx_idem; f_equal.
       destruct n; [rewrite !approx_0; auto|].
       setoid_rewrite approx_later.
       etransitivity; [rewrite <- approx_oo_approx' with (n' := S n)|]; auto.
-    + setoid_rewrite fview_shift_nonexpansive.
-      rewrite !approx_idem, protocol_A_super_non_expansive; auto.
   - rewrite !approx_allp by auto; f_equal; extensionality.
     rewrite !approx_allp by auto; f_equal; extensionality.
     setoid_rewrite approx_imp; f_equal; f_equal.
@@ -448,7 +458,7 @@ Qed.
 Next Obligation.
 Proof.
   repeat intro.
-  destruct x as (((((((((?, ?), ?), ?), ?), ?), ?), ?), ?), ?); simpl.
+  destruct x as ((((((((((?, ?), ?), ?), ?), ?), ?), ?), ?), ?), ?); simpl.
   rewrite !approx_exp; apply f_equal; extensionality.
   rewrite !approx_exp; apply f_equal; extensionality.
   unfold PROPx; simpl; rewrite !approx_andp; f_equal.
@@ -457,5 +467,3 @@ Proof.
 Qed.
 
 End atomics.
-
-End inv.
